MemoryModel.thy
@@ -1,0 +1,144 @@
+theory MemoryModel
+  imports Result
+begin
+
+section "Definitions"
+
+
+subsection "Types"
+
+datatype 'a memory_value = mem_unset | mem_val 'a | mem_freed
+type_synonym 'a memory_model = "'a memory_value list"
+type_synonym memory_model_address = nat
+
+
+subsection "Operations"
+
+definition allocate_memory :: "'a memory_model \<Rightarrow> ('a memory_model * memory_model_address)" where
+  "allocate_memory m = (m@[mem_unset], length m)"
+
+definition valid_memory_address :: "'a memory_model \<Rightarrow> memory_model_address \<Rightarrow> bool" where
+  "valid_memory_address m a = (a < length m \<and> m!a \<noteq> mem_freed)"
+
+definition get_memory :: "'a memory_model \<Rightarrow> memory_model_address \<Rightarrow> 'a result" where
+  "get_memory m a =
+    (if valid_memory_address m a then
+      (case (m!a) of
+        mem_unset \<Rightarrow> err uninitialized_address
+      | mem_val v \<Rightarrow> ok v
+      | mem_freed \<Rightarrow> err unallocated_address
+    ) else err unallocated_address)"
+
+definition set_memory :: "'a memory_model \<Rightarrow> memory_model_address \<Rightarrow> 'a \<Rightarrow> 'a memory_model result" where
+  "set_memory m a v = (if valid_memory_address m a then ok (m[a:=(mem_val v)]) else err unallocated_address)"
+
+definition free_memory :: "'a memory_model \<Rightarrow> memory_model_address \<Rightarrow> 'a memory_model result" where
+  "free_memory m a = (if valid_memory_address m a then ok (m[a:=mem_freed]) else err unallocated_address)"
+
+definition empty_memory_model :: "'a memory_model" where
+  "empty_memory_model = []"
+
+
+
+section "Lemmas"
+
+
+subsection "Empty memory"
+
+lemma memory_empty_get: "get_memory empty_memory_model a = err unallocated_address"
+  unfolding empty_memory_model_def get_memory_def valid_memory_address_def
+  by simp
+
+lemma memory_empty_invalid: "\<not>valid_memory_address empty_memory_model a"
+  unfolding empty_memory_model_def valid_memory_address_def
+  by simp
+
+lemma memory_empty_set: "set_memory empty_memory_model a v = err unallocated_address"
+  unfolding empty_memory_model_def set_memory_def valid_memory_address_def
+  by simp
+
+
+subsection "Allocate"
+
+lemma memory_allocate_get_uninitialized: "allocate_memory m = (m', i) \<longrightarrow> get_memory m' i = err uninitialized_address"
+  unfolding allocate_memory_def get_memory_def valid_memory_address_def 
+  by auto
+
+lemma memory_allocate_validity: "(m', i) = allocate_memory m \<longrightarrow> \<not>valid_memory_address m i \<and> valid_memory_address m' i"
+  unfolding allocate_memory_def valid_memory_address_def
+  by simp
+
+(* Removed due to free *)
+(*lemma memory_valid_suc: "valid_memory_address s (Suc i) \<longrightarrow> valid_memory_address s i"
+  using valid_memory_address_def
+  by simp*)
+
+lemma memory_set_unallocated: "\<not>valid_memory_address m i \<longrightarrow> set_memory m i v = err unallocated_address"
+  unfolding set_memory_def
+  by simp
+
+lemma memory_set_ok_valid: "set_memory m i v = ok m' \<longrightarrow> valid_memory_address m' i \<and> valid_memory_address m i"
+  unfolding set_memory_def valid_memory_address_def
+  by auto
+
+lemma memory_get_ok_valid: "get_memory m a = ok v \<longrightarrow> valid_memory_address m a"
+  unfolding get_memory_def valid_memory_address_def
+  by simp
+
+(* GET (PUT X) = X *)
+lemma memory_set_get: "set_memory m i v = ok m' \<longrightarrow> get_memory m' i = ok v"
+  unfolding valid_memory_address_def set_memory_def get_memory_def
+  by auto
+
+(*PUT (PUT X) Y = Y*)
+lemma memory_set_set_get: "set_memory m i v = ok m' \<longrightarrow> set_memory m' i v' = ok m'' \<longrightarrow> get_memory m'' i = ok v'"
+  unfolding valid_memory_address_def set_memory_def get_memory_def
+  by auto
+
+(*PUT (GET I) = ID*)
+lemma memory_get_set_id: "get_memory m i = ok v \<longrightarrow> set_memory m i v = ok m' \<longrightarrow> m = m'"
+  unfolding set_memory_def get_memory_def
+  using list_update_id memory_value.exhaust
+  by (metis memory_value.simps(10,8,9) result.distinct(1) result.inject(1))
+
+(*GET a1, PUT a2, GET a1*)
+lemma memory_set_independent: "a1 \<noteq> a2 \<longrightarrow> get_memory m a1 = ok v1 \<longrightarrow> set_memory m a2 v2 = ok m' \<longrightarrow> get_memory m' a1 = ok v1"
+  unfolding get_memory_def set_memory_def valid_memory_address_def
+  by auto
+
+(*VALID a1 \<rightarrow> ALLOC \<rightarrow> VALID a1*)
+lemma memory_valid_alloc_valid: "valid_memory_address m a \<longrightarrow> allocate_memory m = (m', a') \<longrightarrow> valid_memory_address m' a"
+  unfolding valid_memory_address_def allocate_memory_def
+  using nth_append_left
+  by fastforce
+
+(*GET a1 = (ALLOC, GET a1)*)
+lemma memory_alloc_get_eq: "get_memory m a = ok v \<longrightarrow> allocate_memory m = (m', a') \<longrightarrow> get_memory m' a = ok v"
+  using nth_append_left memory_get_ok_valid
+  unfolding get_memory_def allocate_memory_def valid_memory_address_def
+  by force
+
+
+lemma memory_free_get: "free_memory m a = ok m' \<longrightarrow> get_memory m' a = err unallocated_address"
+  unfolding get_memory_def free_memory_def valid_memory_address_def
+  by auto
+
+lemma memory_free_set: "free_memory m a = ok m' \<longrightarrow> set_memory m' a v = err unallocated_address"
+  unfolding set_memory_def free_memory_def valid_memory_address_def
+  by auto
+
+lemma memory_free_invalid: "free_memory m a = ok m' \<longrightarrow> \<not>valid_memory_address m' a \<and> valid_memory_address m a"
+  unfolding free_memory_def valid_memory_address_def
+  by auto
+
+lemma memory_free_independent_valid: "valid_memory_address m a \<longrightarrow> free_memory m a' = ok m' \<longrightarrow> a \<noteq> a' \<longrightarrow> valid_memory_address m' a"
+  unfolding get_memory_def free_memory_def valid_memory_address_def
+  by auto
+
+lemma memory_free_independent_get: "get_memory m a = ok v \<longrightarrow> free_memory m a' = ok m' \<longrightarrow> a \<noteq> a' \<longrightarrow> get_memory m' a = ok v"
+  unfolding free_memory_def get_memory_def valid_memory_address_def
+  using length_list_update nth_list_update result.distinct(1) result.inject(1)
+  by metis
+
+
+end
