RegisterModel.thy
@@ -1,0 +1,55 @@
+theory RegisterModel
+  imports "HOL-Library.Mapping" Result
+begin
+
+section "Definitions"
+
+
+subsection "Types"
+
+type_synonym register_name = string
+type_synonym 'a register_model = "(register_name, 'a) mapping"
+
+
+subsection "Operations"
+
+definition get_register :: "'a register_model \<Rightarrow> register_name \<Rightarrow> 'a result" where
+  "get_register r n = (case Mapping.lookup r n of None \<Rightarrow> err unknown_register | Some v \<Rightarrow> ok v)"
+
+definition set_register :: "'a register_model \<Rightarrow> register_name \<Rightarrow> 'a \<Rightarrow> 'a register_model result" where
+  "set_register r n v = (case Mapping.lookup r n of None \<Rightarrow> ok (Mapping.update n v r) | Some _ \<Rightarrow> err register_override)"
+
+definition empty_register_model :: "'a register_model" where
+  "empty_register_model = Mapping.empty"
+
+
+
+section "Lemmas"
+
+lemma register_empty_get: "get_register empty_register_model n = err unknown_register"
+  unfolding get_register_def empty_register_model_def
+  by auto
+
+lemma register_set_ok_unknown: "set_register r n v = ok r' \<longrightarrow> get_register r n = err unknown_register"
+  unfolding set_register_def get_register_def option.case_eq_if
+  by simp
+
+lemma register_get_set_get: "get_register r n = ok v \<longrightarrow> set_register r n' v' = ok r' \<longrightarrow> get_register r' n = ok v"
+  unfolding get_register_def set_register_def option.case_eq_if
+  using lookup_update' result.distinct(2) result.simps(1)
+  by metis
+
+lemma register_set_get: "set_register r n v = ok r' \<longrightarrow> get_register r' n = ok v"
+  using register_set_ok_unknown
+  unfolding set_register_def get_register_def option.case_eq_if
+  by auto
+
+lemma register_get_ok_set: "get_register r n = ok v \<longrightarrow> set_register r n v' = err register_override"
+  unfolding set_register_def get_register_def option.case_eq_if
+  by simp
+
+lemma register_set_set: "set_register r n v = ok r' \<longrightarrow> set_register r' n v' = err register_override"
+  unfolding set_register_def option.case_eq_if
+  by auto
+
+end
